src/sim/Simulation.v
@@ -1,6 +1,7 @@
 Require Import sflib.
 
 Require Import Event.
+Require Import Memory.
 Require Import Configuration.
 Require Import Program.
 
@@ -17,19 +18,7 @@ Inductive tausteps: forall (src:Configuration.t) (src':Configuration.t), Prop :=
     tausteps src src''
 .
 
-Inductive srcsteps: forall (src:Configuration.t) (e:option Event.t) (src':Configuration.t), Prop :=
-| srcsteps_stationary
-    src src'
-    (TAU: tausteps src src'):
-    srcsteps src None src'
-| srcsteps_progress
-    src src' src'' e
-    (TAU: tausteps src src')
-    (PROGRESS: Configuration.step src' e src''):
-    srcsteps src e src''
-.
-
-(* TODO: proper use of indexes *)
+(* TODO: liveness *)
 Module Simulation.
   Section Simulation.
     Variable (prog_src prog_tgt:Program.syntax).
@@ -38,20 +27,101 @@ Module Simulation.
     Definition LOAD: Prop := sim (Configuration.load prog_src) (Configuration.load prog_tgt).
 
     Definition STEP: Prop :=
-      forall src tgt e tgt'
-        (SIM: sim src tgt)
-        (STEP: Configuration.step tgt e tgt'),
-      exists src',
-        <<STEP: srcsteps src e src'>> /\
-                <<SIM: sim src' tgt'>>.
+      forall src0 tgt0 e tgt2
+        (SIM: sim src0 tgt0)
+        (STEP: Configuration.step tgt0 e tgt2),
+      exists src1 src2,
+        <<INTERNAL: Configuration.internal_steps src0 src1>> /\
+        <<STEP: Configuration.step src1 e src2>> /\
+        <<SIM: sim src2 tgt2>>.
 
     Definition TERMINAL: Prop :=
+      forall src0 tgt0
+        (SIM: sim src0 tgt0)
+        (TERM: Configuration.is_terminal tgt0),
+      exists src1,
+        <<INTERNAL: Configuration.internal_steps src0 src1>> /\
+        <<TERM: Configuration.is_terminal src1>>.
+
+    Definition FEASIBLE: Prop :=
       forall src tgt
         (SIM: sim src tgt)
-        (TERM: Configuration.is_terminal tgt),
-      exists src',
-        <<STEP: tausteps src src'>> /\
-        <<TERM: Configuration.is_terminal src'>>.
+        (FEASIBLE: Configuration.feasible tgt),
+        Configuration.feasible src.
+
+    Definition BASE_STEP: Prop :=
+      forall src0 tgt0 tgt2
+        (SIM: sim src0 tgt0)
+        (STEP: Configuration.base_step tgt0 tgt2),
+      exists src1 src2,
+        <<INTERNAL: Configuration.internal_steps src0 src1>> /\
+        <<STEP: Configuration.internal_step src1 src2>> /\
+        <<SIM: sim src2 tgt2>>.
+
+    Definition INCEPTION_STEP: Prop :=
+      forall src0 src1
+        c0_tgt th0_tgt m0_tgt
+        c1_tgt th1_tgt m1_tgt
+        inception
+        (STEPS_TGT: Configuration.internal_steps (Configuration.mk c0_tgt th0_tgt m0_tgt) (Configuration.mk c1_tgt th1_tgt m1_tgt))
+        (INCEPTION: Memory.inception m1_tgt inception)
+        (CONSISTENT: Memory.consistent (Memory.mk m0_tgt.(Memory.buffers) (InceptionSet.add inception m0_tgt.(Memory.inceptions))))
+        (SIM0: sim src0 (Configuration.mk c0_tgt th0_tgt m0_tgt))
+        (STEPS_SRC: Configuration.internal_steps src0 src1)
+        (SIM1: sim src1 (Configuration.mk c1_tgt th1_tgt m1_tgt)),
+      exists src1 src2,
+        <<INTERNAL: Configuration.internal_steps src0 src1>> /\
+        <<STEP: Configuration.internal_step src1 src2>> /\
+        <<SIM: sim src2 (Configuration.mk c0_tgt th0_tgt (Memory.mk m0_tgt.(Memory.buffers) (InceptionSet.add inception m0_tgt.(Memory.inceptions))))>>.
+
+    Definition SYSCALL_STEP: Prop :=
+      forall src0 tgt0 e tgt2
+        (SIM: sim src0 tgt0)
+        (STEP: Configuration.step tgt0 (Some e) tgt2),
+      exists src1 src2,
+        <<INTERNAL: Configuration.internal_steps src0 src1>> /\
+        <<STEP: Configuration.step src1 (Some e) src2>> /\
+        <<SIM: sim src2 tgt2>>.
+
+    Lemma internal_step (B:BASE_STEP) (I:INCEPTION_STEP):
+      forall src0 tgt0 tgt2
+        (SIM: sim src0 tgt0)
+        (STEP: Configuration.internal_step tgt0 tgt2),
+      exists src1 src2,
+        <<INTERNAL: Configuration.internal_steps src0 src1>> /\
+        <<STEP: Configuration.internal_step src1 src2>> /\
+        <<SIM: sim src2 tgt2>>
+    with internal_steps (B:BASE_STEP) (I:INCEPTION_STEP):
+      forall src0 tgt0 tgt1
+        (SIM: sim src0 tgt0)
+        (STEP: Configuration.internal_steps tgt0 tgt1),
+      exists src1,
+        <<INTERNAL: Configuration.internal_steps src0 src1>> /\
+        <<SIM: sim src1 tgt1>>.
+    Proof.
+      - i. inv STEP0.
+        + exploit B; eauto.
+        + exploit internal_steps; eauto. i. des.
+          exploit I; eauto.
+      - i. revert src0 SIM. induction STEP0.
+        + i. exists src0. splits; eauto. econs.
+        + i. exploit internal_step; eauto. i. des.
+          exploit IHSTEP0; eauto. i. des.
+          exists src3. splits; auto.
+          eapply Configuration.internal_steps_append; eauto.
+          eapply Configuration.internal_steps_append; eauto.
+          econs; eauto. econs.
+    Qed.
+
+    Lemma step_lemma (F:FEASIBLE) (B:BASE_STEP) (I:INCEPTION_STEP) (S:SYSCALL_STEP): STEP.
+    Proof.
+      ii. inv STEP0.
+      - exploit internal_step; eauto. i. des.
+        eexists _, _. splits; eauto.
+        econs; eauto.
+      - exploit S; eauto.
+        econs; eauto.
+    Qed.
   End Simulation.
 
   Structure t (prog_src prog_tgt:Program.syntax) := mk {
